\documentclass[12pt]{article}

\input{hw-preamble}

\begin{document}
\thispagestyle{empty}
\hw{3}{5 November 2023}

\problem Proof by resolution.
\solution Translate the following into first-order logic.
\begin{flalign*}
    \text{Every kid likes Snoopy} \quad                                    & \quad \forall x(K(x)\rightarrow L(x, Snoopy))                                 \\
    \text{Everyone who likes Snoopy likes all beagles} \quad               & \quad \forall x (L(x, Snoopy)\rightarrow (\forall y B(y)\rightarrow L(x, y))) \\
    \text{Underdog is a beagle, and Underdog is a superhero} \quad         & \quad B(Underdog)\land S(Underdog)                                            \\
    \text{Every superhero can fly or time travel} \quad                    & \quad \forall x(S(x)\rightarrow (F(x)\lor T(x)))                              \\
    \text{No beagle can time travel} \quad                                 & \quad \lnot\exists x(B(x)\land T(x))                                          \\
    \text{Garfield does not like all things that can fly} \quad            & \quad \lnot\forall x(F(x)\rightarrow L(Garfield, x))                          \\
    \text{Garfield is not a kid. (goal that will be negated latter)} \quad & \quad \lnot K(Garfield)
\end{flalign*}

\noindent
Convert the resulting formulas into a canonical form
\begin{enumerate}
    \item $\forall x(K(x)\rightarrow L(x, Snoopy))$\\
          $\forall x(\lnot K(x)\lor L(x,Snoopy))$

    \item $\forall x (L(x, Snoopy)\rightarrow \forall y (B(y)\rightarrow L(x, y)))$\\
          $\forall x\forall y(L(x, Snoopy)\rightarrow (B(y)\rightarrow L(x,y)))$ \\
          $\forall x\forall y(L(x, Snoopy)\rightarrow (\lnot B(y)\lor L(x,y)))$ \\
          $\forall x\forall y(\lnot L(x, Snoopy)\lor (\lnot B(y)\lor L(x,y)))$ \\
          $\forall x\forall y(\lnot L(x, Snoopy)\lor \lnot B(y)\lor L(x,y))$

    \item $B(Underdog)\land S(Underdog)$\\
          $B(Underdog)$\\
          $S(Underdog)$

    \item $\forall x(S(x)\rightarrow (F(x)\lor T(x)))$\\
          $\forall x(\lnot S(x)\lor (F(x)\lor T(x)))$\\
          $\forall x(\lnot S(x)\lor F(x)\lor T(x))$

    \item $\lnot\exists x(B(x)\land T(x))$\\
          $\forall x\lnot(B(x)\land T(x))$\\
          $\forall x(\lnot B(x)\lor \lnot T(x))$

    \item $\lnot\forall x(F(x)\rightarrow L(Garfield, x))$\\
          $\lnot\forall x(\lnot F(x)\lor L(Garfield, x))$\\
          $\exists x (F(x)\land \lnot L(Garfield, x)$\\
          $F(\alpha)\land \lnot L(Garfield, \alpha)$\\
          $F(\alpha)$\\
          $\lnot L(Garfiled, \alpha)$

    \item Negated goal: $K(Garfield)$
\end{enumerate}

\noindent
Resolving negated goal clause with $\lnot K(x)\lor L(x,Snoopy)$\\
$\sigma=\{x/Garfield\}$\\
$L(Garfield, Snoopy)$

\noindent
Resolving $L(Garfield, Snoopy)$ with $\forall x\forall y(\lnot L(x, Snoopy)\lor \lnot B(y)\lor L(x,y))$\\
$\sigma=\{x/Garfield\}$\\
$\lnot B(y)\lor L(Garfield,y)$

\noindent
Resolving $\lnot B(y)\lor L(Garfield,y)$ with $B(Underdog)$\\
$\sigma=\{y/Underdog\}$\\
$L(Garfield,Underdog)$

\noindent
Resolving $L(Garfield,Underdog)$ with $\lnot L(Garfield,\alpha)$\\
$\sigma=\{\alpha/Underdog\}$\\
NULL Clause

\noindent
The statement is proven $\qed$

\newpage
\problem The resolution theorem prover.

\solution The resolution theorem prover is included in the submission folder.

\problem Prolog

\solution
The knowledge base is included in the submission folder as requested.\\
The queries are translated to prolog as follows:
\begin{minted}{prolog}
grandparent(charles, X).
brother(william, X), spouse(X, Y).
uncle(X, charlotte).
aunt(X, archie).
nephew(X, harry).
stepmother(X, william).
sibling(X, Y).
cousin(X, Y), female(X).
niece(X, Y).
\end{minted}

\noindent
The answers as determined by the Knowledge Base are as follows:
\begin{minted}{prolog}
X = george
X = harry, Y = meghan
X = harry
X = catherine
X = george
X = camila
X = william, Y = harry
X = charlotte, Y = archie
X = charlotte, Y = harry
\end{minted}
\end{document}

